---
layout: page
title: Section 1.2 Calculus 2
description: Hyperbolic Functions
---

[Back to Table of Contents](../..)

---

## 1.2 Hyperbolic Functions

### 1.2.1 Hyperbolic Sine and Cosine

<iframe src="https://www.youtube.com/embed/J78Ido7MOxE" frameborder="0" allowfullscreen></iframe>

- Exponential functions are used to define the hyperbolic functions,
  which behave like trigonometric functions in many ways.
    - \\(\sinh x = \frac{e^x-e^{-x}}{2}\\)
    - \\(\cosh x = \frac{e^x+e^{-x}}{2}\\)
- **Example** Evaluate \\(\sinh(0)\\) and \\(\cosh(0)\\).
- **Example** Evaluate \\(\cosh(\ln 4)\\).
- **Example** Prove that \\(\sinh(2x)=2\sinh(x)\cosh(x)\\).

\\(\newcommand{\sech}{\mathrm{sech}\,}\\)
\\(\newcommand{\csch}{\mathrm{csch}\,}\\)

### 1.2.2 Other Hyperbolic Functions

<iframe src="https://www.youtube.com/embed/5pHJkJoPSiA" frameborder="0" allowfullscreen></iframe>

- The other hypberbolic functions are defined the same way their
  trig counterparts are, and have similar properties.
    - \\(\tanh x = \frac{\sinh x}{\cosh x} = \frac{e^x-e^{-x}}{e^x+e^{-x}}\\)
    - \\(\coth x = \frac{\cosh x}{\sinh x} = \frac{e^x+e^{-x}}{e^x-e^{-x}}\\)
    - \\(\sech x = \frac{1}{\cosh x}=\frac{2}{e^x+e^{-x}}\\)
    - \\(\csch x = \frac{1}{\sinh x}=\frac{2}{e^x-e^{-x}}\\)
- **Example** Evaluate \\(\sech(-\ln 2)\\).
- **Example** Prove that \\(\tanh^2(x)=1-\sech^2(x)\\).


### 1.2.3 Derivatives and Integrals of Hyperbolic Functions

<iframe src="https://www.youtube.com/embed/8WSn1tyUE90" frameborder="0" allowfullscreen></iframe>

- Their derivatives also behave similarly.
    - \\(\frac{d}{dx}[\sinh x] = \cosh x\\)
    - \\(\frac{d}{dx}[\cosh x] = \sinh x\\)
    - \\(\frac{d}{dx}[\tanh x] = \sech^2 x\\)
    - \\(\frac{d}{dx}[\coth x] = -\csch^2 x\\)
    - \\(\frac{d}{dx}[\sech x] = -\sech x\tanh x\\)
    - \\(\frac{d}{dx}[\csch x] = -\csch x\coth x\\)
- **Example**
  Use their definitions to prove that \\(\frac{d}{dx}[\cosh x]=\sinh x\\).
- **Example**
  Use their definitions to prove that \\(\frac{d}{dx}[\coth x]=\csch^2 x\\).
- **Example**
  Compute \\(\frac{d}{dx}[\sinh(2x)+\coth(x^2)]\\).
- Their integral formulas may be found by just reversing the equations.
    - \\(\int \cosh x\,dx = \sinh x + C \\)
    - \\(\int \sinh x\,dx = \cosh x + C \\)
    - \\(\int \sech^2 x\,dx = \tanh x + C \\)
    - \\(\int \csch^2 x\,dx = -\coth x + C \\)
    - \\(\int\sech x\tanh x\,dx = -\sech x + C \\)
    - \\(\int\csch x\coth x\,dx = -\csch x + C \\)
- **Example**
  Find \\(\int (4\csch^2 x-3\sinh x)\,dx\\).

---

### Review Exercises

1.  Evaluate \\(\sinh(\ln 6)\\).
3.  Prove that \\(\cosh (2x) = \cosh^2 x + \sinh^2 x\\).
3.  Prove that \\(\cosh^2 x - \sinh^2 x = 1\\).
4.  Evaluate \\(\tanh(\ln 3)\\).
5.  Simplify \\(\sinh(x)\coth(x)\cosh(x)-\frac{1}{\csch^2(x)}\\).
    (Hint: convert everything to \\(\sinh x\\) and \\(\cosh x\\).)
6.  Prove that \\(\frac{d}{dx}[\sinh x] = \cosh x\\).
7.  Prove that \\(\frac{d}{dx}[\sech x] = -\sech x\tanh x\\).
    (Hint: use the fact that \\(\frac{d}{dx}[\cosh x] = \sinh x\\).)
8.  Compute \\(\frac{d}{dx}[\tanh(3x)-\sech(\ln x)]\\).
9.  Find \\(\int (3\csch x\coth x - 2\sinh x)\,dx\\).
10. (Optional)
    Let \\(\sinh^{\leftarrow}(x)\\) be the inverse function of
    \\(\sinh(x)\\). Use the facts
    \\(\frac{d}{dx}[f^{\leftarrow}(x)]=\frac{1}{f'(f^{\leftarrow}(x))}\\)
    and \\(\cosh^2 x-\sinh^2 x = 1\\) to prove that
    \\(\frac{d}{dx}[\sinh^{\leftarrow}(x)]=\frac{1}{\sqrt{1+x^2}}\\).
11. Prove that \\(\sinh^{\leftarrow}(x)=\ln(\sqrt{x^2+1}+x)\\).
12. Evaluate \\(\cosh(\ln 2)\\).
13. Differentiate \\(f(x)=\tanh(x^2)-\cosh(2x+1)\\).

### Solutions

- [Solutions 1-11](/resources/calculus2/solutions/1.2.a.pdf)
- [Solutions 12-13](/resources/calculus2/solutions/1.2.b.pdf)

---



### Textbook References

- University Calculus: Early Transcendentals (3rd Ed)
    - 7.3
